\documentclass[preview]{standalone}

\usepackage[english]{babel}
\usepackage{amsmath}
\usepackage{amssymb}
\usepackage{dsfont}
\usepackage{setspace}
\usepackage{tipa}
\usepackage{relsize}
\usepackage{textcomp}
\usepackage{mathrsfs}
\usepackage{calligra}
\usepackage{wasysym}
\usepackage{ragged2e}
\usepackage{physics}
\usepackage{xcolor}
\usepackage{microtype}
\DisableLigatures{encoding = *, family = * }
%\usepackage[UTF8]{ctex}
\linespread{1}

\begin{document}

\centering \textbf{First sum}: $\displaystyle\sum_{n=0}^{\infty}(-1)^n$ = $1-1+1-1+1 \dots$$ = \frac{1}{2}$

\end{document}
